1 admit solved, 1 remains in map ~ pmap

src/Concurrent/Experimental/MapPmap.v
@@ -3,70 +3,191 @@ From CoreErlang.FrameStack Require Import SubstSemantics Examples.
 
 Import ListNotations.
 
-(*
+Lemma etherAdd_lookup :
+  forall ιs ιd ι1 ι2 t l eth,
+    etherAdd ιs ιd t eth !! (ι1, ι2) = Some l ->
+      eth !! (ι1, ι2) = Some l \/ 
+      (ι1 = ιs /\ ι2 = ιd /\ exists l', l = l' ++ [t]).
+Proof.
+  intros. destruct (decide ((ιs, ιd) = (ι1, ι2))).
+  * inv e. right. intuition.
+    unfold etherAdd in H. case_match; setoid_rewrite lookup_insert in H; inv H.
+    1: by eexists.
+    1: by exists [].
+  * unfold etherAdd in H. case_match; setoid_rewrite lookup_insert_ne in H; auto.
+Qed.
 
-This does not work this way. We have to either remove the side conditions, 
-or add more.
 
+Definition appearsOnlyAsSourceAndNoLink (ι : PID) (eth : Ether) : Prop :=
+  ¬isTargetedEther ι eth /\
+  (forall (ιs ιd : PID) (t : list Signal),
+         eth !! (ιs, ιd) = Some t -> ι ∉ flat_union usedPIDsSignal t) /\
+  (forall ιd l, eth !! (ι, ιd) = Some l -> SLink ∉ l /\ forall r b, SExit r b ∉ l).
+
+Theorem appearsOnlyAsSource_preserved :
+  forall A B ι a O,
+    A -[a | ι]ₙ-> B with O ->
+    forall ιs, appearsOnlyAsSourceAndNoLink ιs A.1 ->
+      ¬ isUsedPool ιs A.2 ->
+      Some ιs ≠ spawnPIDOf a ->
+      appearsOnlyAsSourceAndNoLink ιs B.1 /\ ¬isUsedPool ιs B.2.
+Proof with by setoid_rewrite lookup_insert.
+  intros. inv H; simpl in *.
+  * clear H2. destruct H0.
+    split. split. 2: split.
+    - intro. apply H. apply isTargetedEther_etherAdd_rev in H2. assumption.
+      intro. subst. apply H1. right. exists ι, p. split. auto...
+      inv H3; simpl in *.
+      1-4: set_solver.
+      apply elem_of_union_list. exists ({[ιs]} ∪ usedPIDsVal reason).
+      split. 2: set_solver.
+      apply elem_of_elements, elem_of_map_to_set. do 2 eexists. split. 2: reflexivity.
+      assumption.
+    - intros. apply etherAdd_lookup in H2 as H2'. destruct H2'.
+      + by apply H0 in H4.
+      + destruct_hyps; subst.
+        intro.
+        assert (ιs ∈ usedPIDsSignal t). {
+          unfold etherAdd in H2. case_match; setoid_rewrite lookup_insert in H2.
+          ** inv H2. apply app_inv_tail in H8. subst.
+             apply H0 in H5. rewrite flat_union_app in H4. simpl in H4.
+             set_solver.
+          ** inv H2. destruct x; inv H8. 2: { destruct x; inv H9. }
+             set_solver.
+        }
+        apply H1. right. exists ι, p. split. auto...
+        inv H3; simpl in *.
+        1-4: set_solver.
+        apply elem_of_union_list. exists ({[ι']} ∪ usedPIDsVal reason).
+        split. 2: set_solver.
+        apply elem_of_elements, elem_of_map_to_set. do 2 eexists. split. 2: reflexivity.
+        assumption.
+    - destruct H0. intros. apply etherAdd_lookup in H4 as H4'.
+      destruct H4'.
+      + by apply H2 in H5.
+      + destruct_hyps; subst.
+        assert (SLink ≠ t /\ forall r b, SExit r b <> t). {
+          inv H3; auto; exfalso;
+          apply H1; left...
+        }
+        unfold etherAdd in H4. case_match; setoid_rewrite lookup_insert in H4.
+        ** inv H4. apply app_inv_tail in H8. subst.
+           apply H2 in H6. set_solver.
+        ** inv H4. destruct x; inv H8. 2: { destruct x; inv H9. }
+           set_solver.
+    - intro. apply H1. apply isUsedPool_insert_1 in H2.
+      apply isUsedPool_insert_2. intuition.
+      inv H3; simpl in *.
+      1-4: do 2 right; set_solver.
+      apply elem_of_union_list in H2. destruct_hyps.
+      apply elem_of_elements, elem_of_map_to_set in H0; destruct_hyps. subst.
+      apply lookup_delete_Some in H0 as [? ?].
+      do 2 right. apply elem_of_union_list. exists ({[x0]} ∪ usedPIDsVal x1). split.
+      2: assumption.
+      apply elem_of_elements, elem_of_map_to_set. do 2 eexists. split. 2: reflexivity.
+      assumption.
+  * destruct H0. split. split. 2: split.
+    - intro. apply H. eapply isTargetedEther_etherPop_rev; eassumption.
+    - intros. unfold etherPop in H3. repeat case_match; try congruence. inv H3.
+      apply H0 in H6. simpl in H6.
+      destruct (decide ((ι1, ι) = (ιs0, ιd))).
+      + inv e. setoid_rewrite lookup_insert in H5. inv H5.
+        set_solver.
+      + setoid_rewrite lookup_insert_ne in H5; auto.
+        by apply H0 in H5.
+    - intros. unfold etherPop in H3. repeat case_match; try congruence. inv H3.
+      destruct H0 as [_ H0].
+      destruct (decide ((ι1, ι) = (ιs, ιd))).
+      + inv e. setoid_rewrite lookup_insert in H5. inv H5.
+        apply H0 in H6. set_solver.
+      + setoid_rewrite lookup_insert_ne in H5; auto.
+        by apply H0 in H5.
+    - intro. apply H1. apply isUsedPool_insert_1 in H5.
+      apply isUsedPool_insert_2. destruct H5. 1: intuition. destruct H5. 1: intuition.
+      unfold etherPop in H3. repeat case_match; try congruence. inv H3.
+      destruct H0.
+      specialize (H0 _ _ _ H6).
+      simpl in H0.
+      inv H4; simpl in *; do 2 right.
+      + rewrite flat_union_app in H5. set_solver.
+      (* the following 3 cases can't happen, but only 2 would cause
+         issues (exit convert, link) since those add the source of the
+         signal to the usedPIDsProc *)
+      + set_solver.
+      + apply elem_of_union_list in H5; destruct_hyps.
+        apply elem_of_elements, elem_of_map_to_set in H4; destruct_hyps.
+        subst. apply lookup_gset_to_gmap_Some in H4 as [? ?]. subst.
+        apply elem_of_union in H5 as [|].
+        ** set_solver.
+        ** destruct_or! H12; destruct_hyps; subst; simpl in H5.
+           all: set_solver.
+      + rewrite flat_union_app in H5. simpl in H5.
+        assert (ιs <> ι1). {
+          intro. subst. apply H3 in H6 as [_ ?]. set_solver.
+        }
+        set_solver.
+      + assert (ιs <> ι1). {
+          intro. subst. apply H3 in H6. set_solver.
+        }
+        set_solver.
+      + set_solver.
+  * split. 1: assumption.
+    eapply not_isUsedPool_step. eassumption.
+    2: { eapply n_other. exact H3. assumption. }
+    destruct_or! H4; subst; simpl. 1,3: set_solver.
+    intro. apply H1. apply elem_of_singleton in H. subst. left...
+  * split. 1: assumption.
+    eapply not_isUsedPool_step.
+    eassumption. 2: eapply n_spawn; try eassumption.
+    assert (ιs <> ι') by congruence.
+    assert (ιs ∉ usedPIDsVal v1 ∪ usedPIDsVal v2). {
+      intro. apply H1. right. exists ι, p. split. auto...
+      inv H8; simpl; simpl in H9; set_solver.
+    }
+    set_solver.
+  Unshelve.
+    exact O.
+    exact ether.
+Qed.
+
+Print appearsEther.
 Unset Guard Checking.
 Theorem almost_terminated_bisim :
   forall O A mb flag ι vs,
-    ¬isTargetedEther ι A.1 ->
+    appearsOnlyAsSourceAndNoLink ι A.1 ->
     ¬isUsedPool ι A.2 ->
     ι ∉ O ->
     A ~ (A.1, ι ↦ inl ([], RValSeq vs, mb, ∅, flag) ∥ A.2) observing O.
 Proof with left; by setoid_rewrite lookup_insert.
   cofix IH. intros * Heth HΠ HO. constructor; intros.
   2,4: exists source; do 2 eexists; split; [apply n_refl|]; simpl; apply option_biforall_refl; intros; apply Signal_eq_refl.
-  * inv H; simpl in *.
-    - do 2 eexists. split.
+  * inversion H; subst; simpl in *.
+    - eapply appearsOnlyAsSource_preserved in H as [H_1 H_2]; try eassumption.
+      2: by simpl.
+      do 2 eexists. split.
       + setoid_rewrite insert_commute. 2: apply not_isUsedPool_insert_1 in HΠ; set_solver.
         eapply n_trans. 2: apply n_refl. by apply n_send.
       + setoid_rewrite insert_commute. 2: apply not_isUsedPool_insert_1 in HΠ; set_solver.
         apply IH; try assumption.
-        ** intro. simpl in *. apply isTargetedEther_etherAdd_rev in H. congruence.
-           intro. subst. apply HΠ. right. exists ι0, p. split.
-           by setoid_rewrite lookup_insert.
-           inv H0; simpl. 1-4: set_solver.
-           apply elem_of_union_list. exists ({[ι]} ∪ usedPIDsVal reason).
-           split. 2: set_solver.
-           apply elem_of_elements, elem_of_map_to_set. exists ι, reason.
-           by split.
-        ** simpl. intro. apply HΠ. apply isUsedPool_insert_1 in H.
-           apply isUsedPool_insert_2. intuition.
-           right. right.
-           inv H0; simpl in *. 1-4: set_solver.
-           apply elem_of_union_list in H; destruct_hyps.
-           apply elem_of_elements, elem_of_map_to_set in H. destruct_hyps.
-           apply lookup_delete_Some in H. destruct_hyps.
-           apply elem_of_union_list. exists ({[x0]} ∪ usedPIDsVal x1). split.
-           2: set_solver.
-           apply elem_of_elements, elem_of_map_to_set.
-           exists x0, x1. by split.
-    - do 2 eexists. split.
+    - eapply appearsOnlyAsSource_preserved in H as [H_1 H_2]; try eassumption.
+      2: by simpl.
+      do 2 eexists. split.
       + setoid_rewrite insert_commute. 2: apply not_isUsedPool_insert_1 in HΠ; set_solver.
         eapply n_trans. 2: apply n_refl. by apply n_arrive.
       + setoid_rewrite insert_commute. 2: apply not_isUsedPool_insert_1 in HΠ; set_solver.
         apply IH; try assumption.
-        ** intro. eapply isTargetedEther_etherPop_rev in H. 2: eassumption.
-           congruence.
-        ** simpl. intro. apply HΠ. apply isUsedPool_insert_1 in H.
-           apply isUsedPool_insert_2. intuition.
-           right. right.
-           inv H1; simpl in *.
-           1-4: set_solver.
-           apply elem_of_union_list in H; destruct_hyps.
-           apply elem_of_elements, elem_of_map_to_set in H. destruct_hyps.
-           apply lookup_delete_Some in H. destruct_hyps.
-           apply elem_of_union_list. exists ({[x0]} ∪ usedPIDsVal x1). split.
-           2: set_solver.
-           apply elem_of_elements, elem_of_map_to_set.
-           exists x0, x1. by split.
-    - do 2 eexists. split.
-      + setoid_rewrite insert_commute. 2: set_solver.
+    - assert (ι <> ι0). {
+        intro. subst. apply HΠ...
+      }
+      do 2 eexists. split.
+      + setoid_rewrite insert_commute. 2: assumption.
         eapply n_trans. 2: apply n_refl. by apply n_other.
-      + setoid_rewrite insert_commute. 2: set_solver.
-        apply IH; try assumption. set_solver.
+      + setoid_rewrite insert_commute. 2: auto.
+        apply IH; try assumption.
+        simpl.
+        eapply not_isUsedPool_step. eassumption. 2: apply n_other; eassumption.
+        destruct_or! H1; subst.
+        all: set_solver.
     - assert (exists fresh, ¬isUsedPool fresh (ι0 ↦ p ∥ Π)
                          /\ ¬appearsEther fresh ether
                          /\ fresh <> ι'
@@ -76,75 +197,112 @@ Proof with left; by setoid_rewrite lookup_insert.
                          /\ ¬ isUsedPool fresh
          (ι' ↦ inl ([], r, emptyBox, if link_flag then {[ι0]} else ∅, false) ∥ ι0 ↦ p' ∥ Π)) as [fresh Hf]. {
         (* freshness *)
-        admit.
+        clear.
+        pose proof (infinite_is_fresh (
+             elements (allPIDsPool (ι0 ↦ p ∥ Π))
+          ++ elements (allPIDsEther ether)
+          ++ [ι']
+          ++ elements O
+          ++ elements (usedPIDsAct (ASpawn ι' v1 v2 link_flag))
+          ++ elements (allPIDsPool (ι ↦ inl ([], RValSeq vs, mb, ∅, flag) ∥ ι0 ↦ p ∥ Π))
+          ++ elements (allPIDsPool (ι' ↦ inl ([], r, emptyBox, if link_flag then {[ι0]} else ∅, false)
+                   ∥ ι0 ↦ p' ∥ Π))
+        )).
+        repeat apply not_elem_of_app in H as [? H].
+        apply not_elem_of_cons in H2 as [H2 _].
+        eexists. split_and!.
+        3: exact H2.
+        3-4: set_solver.
+        2: apply allPIDsEther_does_not_appear_1; set_solver.
+        all: apply allPIDsPool_isNotUsed_1; set_solver.
       }
       destruct_hyps.
       assert (fresh <> ι0) as Hf2. {
-        intro. subst. apply H1...
+        intro. subst. apply H6...
       }
       assert (ι' <> ι0) as Hneq. {
-        intro. subst. apply H4...
+        intro. subst. apply H2...
       }
       assert (fresh <> ι) as Hf. {
-          intro. subst. apply H12...
+        intro. subst. apply H11...
+      }
+      assert (ι' ∉ usedPIDsVal v1 ∪ usedPIDsVal v2 ∪ usedPIDsProc p). {
+        intro. apply H2.
+        right. exists ι0, p. split. by setoid_rewrite lookup_insert.
+        inv H5; simpl in *; set_solver.
+      }
+      assert (renamePIDProc ι' fresh 
+               (inl ([], r, emptyBox, if link_flag then {[ι0]} else ∅, false)) =
+               (inl ([], r, emptyBox, if link_flag then {[ι0]} else ∅, false))) as Hp.
+      {
+        cbn. replace (set_map (renamePIDPID ι' fresh) (if link_flag then {[ι0]} else ∅)) with
+                     (if link_flag then {[ι0]} else ∅ : gset PID). 2: {
+          case_match; auto. setoid_rewrite set_map_singleton_L.
+          clear -Hf2 Hneq. by renamePIDPID_case_match.
         }
-        assert (ι' ∉ usedPIDsVal v1 ∪ usedPIDsVal v2 ∪ usedPIDsProc p). {
-          intro. apply H4.
-          right. exists ι0, p. split. by setoid_rewrite lookup_insert.
-          inv H7; simpl in *; set_solver.
-        }
-        assert (renamePIDProc ι' fresh 
-                 (inl ([], r, emptyBox, if link_flag then {[ι0]} else ∅, false)) =
-                 (inl ([], r, emptyBox, if link_flag then {[ι0]} else ∅, false))) as Hp.
-        {
-          cbn. replace (set_map (renamePIDPID ι' fresh) (if link_flag then {[ι0]} else ∅)) with
-                       (if link_flag then {[ι0]} else ∅ : gset PID). 2: {
-            case_match; auto. setoid_rewrite set_map_singleton_L.
-            clear -Hf2 Hneq. by renamePIDPID_case_match.
+        repeat f_equal.
+        rewrite isNotUsed_renamePID_red. reflexivity.
+        destruct v1; inv H4; cbn.
+        1-8: set_solver.
+        case_match; inv H15. 2: set_solver.
+        simpl. intro. apply subst_usedPIDs in H14; simpl in *.
+        destruct H14; destruct_hyps. set_solver.
+        apply list_subst_idsubst_inl in H14.
+        apply elem_of_app in H14 as [|].
+        * apply elem_of_map_iff in H14; destruct_hyps. destruct x1, p0. subst.
+          simpl in H15. apply elem_of_union in H15 as [|]. 2: set_solver.
+          assert (ι' ∈ flat_union (λ x : nat * nat * Exp, usedPIDsExp x.2) ext). {
+            apply elem_of_flat_union. eexists; split; eassumption.
           }
-          repeat f_equal.
-          rewrite isNotUsed_renamePID_red. reflexivity.
-          destruct v1; inv H6; cbn.
-          1-8: set_solver.
-          case_match; inv H16. 2: set_solver.
-          simpl. intro. apply subst_usedPIDs in H15; simpl in *.
-          destruct H15; destruct_hyps. set_solver.
-          apply list_subst_idsubst_inl in H15.
-          apply elem_of_app in H15 as [|].
-          * apply elem_of_map_iff in H15; destruct_hyps. destruct x1, p0. subst.
-            simpl in H16. apply elem_of_union in H16 as [|]. 2: set_solver.
-            assert (ι' ∈ flat_union (λ x : nat * nat * Exp, usedPIDsExp x.2) ext). {
-              apply elem_of_flat_union. eexists; split; eassumption.
-            }
-            set_solver.
-          * eapply mk_list_usedPIDs in H2.
-            assert (ι' ∈ flat_union usedPIDsVal l). {
-              apply elem_of_flat_union. eexists; split; eassumption.
-            }
-            set_solver.
-        }
-        assert (
-         ι0 ↦ renamePIDProc ι' fresh p' 
-         ∥ fresh
-           ↦ (inl ([], r, emptyBox, if link_flag then {[ι0]} else ∅, false)) ∥ Π .[ ι' ⇔ fresh ]ₚₚ = ι0 ↦ renamePIDProc ι' fresh p' 
-         ∥ fresh
-           ↦ (inl ([], r, emptyBox, if link_flag then {[ι0]} else ∅, false)) ∥ Π
-        ) as HΠ.
-        {
-          apply map_eq. intros.
-          destruct (decide (ι0 = i)).
-          - subst. by setoid_rewrite lookup_insert.
-          - setoid_rewrite lookup_insert_ne; auto.
-            destruct (decide (fresh = i)).
-            + subst. by setoid_rewrite lookup_insert.
-            + setoid_rewrite lookup_insert_ne; auto.
-              admit. (* TODO: later *)
-        }
+          set_solver.
+        * eapply mk_list_usedPIDs in H0.
+          assert (ι' ∈ flat_union usedPIDsVal l). {
+            apply elem_of_flat_union. eexists; split; eassumption.
+          }
+          set_solver.
+      }
+      assert (
+       ι0 ↦ renamePIDProc ι' fresh p' 
+       ∥ fresh
+         ↦ (inl ([], r, emptyBox, if link_flag then {[ι0]} else ∅, false)) ∥ Π .[ ι' ⇔ fresh ]ₚₚ = ι0 ↦ renamePIDProc ι' fresh p' 
+       ∥ fresh
+         ↦ (inl ([], r, emptyBox, if link_flag then {[ι0]} else ∅, false)) ∥ Π
+      ) as HΠ2.
+      {
+        apply map_eq. intros.
+        destruct (decide (ι0 = i)).
+        - subst. by setoid_rewrite lookup_insert.
+        - setoid_rewrite lookup_insert_ne; auto.
+          destruct (decide (fresh = i)).
+          + subst. by setoid_rewrite lookup_insert.
+          + setoid_rewrite lookup_insert_ne; auto.
+            destruct (decide (i = ι')).
+            ** subst.
+               replace (ι') with (renamePIDPID_sym ι' fresh fresh) at 1 by renamePIDPID_sym_case_match.
+               setoid_rewrite lookup_kmap; auto. setoid_rewrite lookup_fmap.
+               assert (fresh ∉ dom Π /\ ι' ∉ dom Π) as [D1 D2]. {
+                 split.
+                 * apply not_isUsedPool_insert_1 in H6. apply H6.
+                 * apply not_isUsedPool_insert_1 in H2. apply H2.
+               }
+               apply not_elem_of_dom in D1, D2. setoid_rewrite D1.
+               by setoid_rewrite D2.
+            ** replace i with (renamePIDPID_sym ι' fresh i) at 1 by renamePIDPID_sym_case_match.
+               setoid_rewrite lookup_kmap; auto. setoid_rewrite lookup_fmap.
+               destruct (Π !! i) eqn:P; setoid_rewrite P. 2: reflexivity.
+               simpl.
+               setoid_rewrite isNotUsed_renamePID_proc. reflexivity.
+               -- intro. apply H2. right. exists i, p0. split. 2: eassumption.
+                  by setoid_rewrite lookup_insert_ne.
+               -- intro. apply H6. right. exists i, p0. split. 2: eassumption.
+                  by setoid_rewrite lookup_insert_ne.
+      }
+      assert (ι <> ι0). 1: intro; subst; apply HΠ...
       exists (renamePIDEther ι' fresh ether, ι ↦ inl ([], RValSeq vs, mb, ∅, flag) ∥ renamePIDPool ι' fresh (
       ι' ↦ inl ([], r, emptyBox, if link_flag then {[ι0]} else ∅, false) ∥ ι0 ↦ p' ∥ Π)), [(renamePIDAct ι' fresh (ASpawn ι' v1 v2 link_flag), ι0)].
       split.
-      + setoid_rewrite (insert_commute _ ι ι0). 2: set_solver.
-        setoid_rewrite (insert_commute _ ι' ι0). 2: set_solver.
+      + setoid_rewrite (insert_commute _ ι ι0). 2: by auto.
+        setoid_rewrite (insert_commute _ ι' ι0). 2: by auto.
         repeat rewrite pool_insert_renamePID.
         replace (renamePIDPID_sym ι' fresh ι0) with ι0.
         replace (renamePIDPID_sym ι' fresh ι') with fresh.
@@ -152,85 +310,148 @@ Proof with left; by setoid_rewrite lookup_insert.
           renamePIDPID_sym_case_match.
         }
         2: {
-          clear -H9 H4 H12. renamePIDPID_sym_case_match.
-          all: exfalso.
-          * apply H4...
-          * apply H12. left.
-            destruct (decide (fresh = ι)).
-            - subst. by setoid_rewrite lookup_insert.
-            - setoid_rewrite lookup_insert_ne; auto. by setoid_rewrite lookup_insert.
+          (* clear -H9 H4 H12. *) renamePIDPID_sym_case_match.
         }
         simpl renamePIDAct.
-        rewrite Hp, HΠ.
+        rewrite Hp, HΠ2.
         replace (renamePIDPID ι' fresh ι') with fresh by renamePIDPID_case_match.
         rewrite isNotUsed_renamePID_val, isNotUsed_renamePID_val.
         2-3: set_solver.
         eapply n_trans. eapply n_spawn; try eassumption.
         ** setoid_rewrite insert_commute. assumption. set_solver.
-        ** eapply renamePID_is_preserved_local with (from := ι') (to := fresh) in H7.
-           simpl in H7.
-           rewrite isNotUsed_renamePID_val, isNotUsed_renamePID_val in H7.
-           replace (renamePIDPID ι' fresh ι') with fresh in H7 by renamePIDPID_case_match.
-           rewrite isNotUsed_renamePID_proc in H7.
-           exact H7.
+        ** eapply renamePID_is_preserved_local with (from := ι') (to := fresh) in H5.
+           simpl in H5.
+           rewrite isNotUsed_renamePID_val, isNotUsed_renamePID_val in H5.
+           replace (renamePIDPID ι' fresh ι') with fresh in H5 by renamePIDPID_case_match.
+           rewrite isNotUsed_renamePID_proc in H5.
+           exact H5.
            1,3-5: set_solver.
-           all: intro; apply H12; right; exists ι0, p; split; [|assumption].
+           all: intro; apply H11; right; exists ι0, p; split; [|assumption].
            all: setoid_rewrite lookup_insert_ne; auto; try by setoid_rewrite lookup_insert.
-           all: set_solver.
         ** rewrite does_not_appear_renamePID_ether; auto.
-           assert (fresh <> ι0). {
-             intro. subst. apply H1...
-           }
-           setoid_rewrite (insert_commute _ ι ι0). 2: set_solver.
-           setoid_rewrite (insert_commute _ fresh ι0). 2: set_solver.
-           setoid_rewrite (insert_commute _ fresh ι). 2: set_solver.
+           setoid_rewrite (insert_commute _ ι ι0). 2: by auto.
+           setoid_rewrite (insert_commute _ fresh ι0). 2: by auto.
+           setoid_rewrite (insert_commute _ fresh ι). 2: by auto.
            apply n_refl.
       + eapply barbedBisim_trans.
         eapply (rename_bisim O _ _ [(ι', fresh)]). cbn. set_solver.
-        simpl. apply IH; simpl. 2: assumption.
-        repeat rewrite pool_insert_renamePID.
-        replace (renamePIDPID_sym ι' fresh ι0) with ι0.
-        replace (renamePIDPID_sym ι' fresh ι') with fresh.
-        2: {
-          renamePIDPID_sym_case_match.
-        }
-        2: {
-          clear -H9 H4 H12. renamePIDPID_sym_case_match.
-          all: exfalso.
-          * apply H4...
-          * apply H12. left.
-            destruct (decide (fresh = ι)).
-            - subst. by setoid_rewrite lookup_insert.
-            - setoid_rewrite lookup_insert_ne; auto. by setoid_rewrite lookup_insert.
-        }
-        rewrite Hp. setoid_rewrite (insert_commute _ fresh ι0); auto.
-        setoid_rewrite HΠ.
-        repeat setoid_rewrite dom_insert_L.
-        set_solver.
+        simpl. apply IH; simpl. 3: assumption.
+        ** by rewrite does_not_appear_renamePID_ether.
+        ** repeat rewrite pool_insert_renamePID.
+           replace (renamePIDPID_sym ι' fresh ι0) with ι0.
+           replace (renamePIDPID_sym ι' fresh ι') with fresh.
+           2: {
+             renamePIDPID_sym_case_match.
+           }
+           2: {
+             renamePIDPID_sym_case_match.
+           }
+           rewrite Hp. setoid_rewrite (insert_commute _ fresh ι0); auto.
+           setoid_rewrite HΠ2.
+           intro. apply HΠ. apply isUsedPool_insert_1 in H15 as [|].
+           setoid_rewrite delete_insert_ne in H15; auto.
+           apply isUsedPool_insert_1 in H15 as [|].
+           -- apply isUsedPool_insert_2. left.
+              setoid_rewrite (delete_notin _ fresh) in H15.
+              assumption.
+              apply not_elem_of_dom.
+              apply not_isUsedPool_insert_1 in H6 as [HD _].
+              clear -HD. set_solver.
+           -- destruct H15. congruence.
+              simpl in H15.
+              right. exists ι0, p. split. by setoid_rewrite lookup_insert.
+              inv H5; simpl in *;
+              destruct (Nat.eqb) in H4; inv H4.
+              2,4: set_solver.
+              ++ repeat rewrite union_empty_r_L in H15.
+                 rewrite union_empty_l_L in H15.
+                 simpl in H15. apply subst_usedPIDs in H15; simpl in *.
+                 destruct H15; destruct_hyps. clear-H4; set_solver.
+                 apply list_subst_idsubst_inl in H4.
+                 apply elem_of_app in H4 as [|].
+                 *** apply elem_of_map_iff in H4; destruct_hyps. destruct x1, p. subst.
+                     simpl in H5. apply elem_of_union in H5 as [|]. 2: clear-H4; set_solver.
+                     assert (ι ∈ flat_union (λ x : nat * nat * Exp, usedPIDsExp x.2) ext). {
+                       apply elem_of_flat_union. eexists; split; try eassumption.
+                     }
+                     clear -H5. set_solver.
+                 *** eapply mk_list_usedPIDs in H0.
+                     assert (ι ∈ flat_union usedPIDsVal l). {
+                       apply elem_of_flat_union. eexists; split; eassumption.
+                     }
+                     clear -H0 H15. set_solver.
+              ++ repeat rewrite union_empty_r_L in H15.
+                 rewrite union_empty_l_L in H15.
+                 simpl in H15. apply elem_of_union in H15 as [H15 | H15].
+                 2: {
+                   clear -H15 H14. set_solver.
+                 }
+                 apply subst_usedPIDs in H15; simpl in *.
+                 destruct H15; destruct_hyps. clear-H4; set_solver.
+                 apply list_subst_idsubst_inl in H4.
+                 apply elem_of_app in H4 as [|].
+                 *** apply elem_of_map_iff in H4; destruct_hyps. destruct x1, p. subst.
+                     simpl in H5. apply elem_of_union in H5 as [|]. 2: clear-H4; set_solver.
+                     assert (ι ∈ flat_union (λ x : nat * nat * Exp, usedPIDsExp x.2) ext). {
+                       apply elem_of_flat_union. eexists; split; try eassumption.
+                     }
+                     clear -H5. set_solver.
+                 *** eapply mk_list_usedPIDs in H0.
+                     assert (ι ∈ flat_union usedPIDsVal l). {
+                       apply elem_of_flat_union. eexists; split; eassumption.
+                     }
+                     clear -H0 H15. set_solver.
+           -- destruct H15. congruence.
+              right. exists ι0. eexists. split. by setoid_rewrite lookup_insert.
+              assert (fresh ∉ usedPIDsProc p). {
+                intro. apply H6. right. do 2 eexists. split.
+                by setoid_rewrite lookup_insert. assumption.
+              }
+              apply renamePID_is_preserved_local with (from := ι') (to := fresh) in H5.
+              2-3: assumption.
+              simpl in H5.
+              rewrite isNotUsed_renamePID_val, isNotUsed_renamePID_val in H5.
+              2-3: clear -H13;set_solver.
+              rewrite renamePIDPID_1 in H5.
+              rewrite isNotUsed_renamePID_proc in H5. 2-3: try assumption; set_solver.
+              eapply not_isUsedProc_step in H5. eassumption. assumption.
+              simpl.
+              intro. apply HΠ. right. do 2 eexists. split. by setoid_rewrite lookup_insert. inv H5; simpl in *; set_solver.
   * destruct (decide (ι0 = ι)).
     {
-      subst. inv H1.
-      * put (lookup ι : ProcessPool -> _) on H4 as D.
-        setoid_rewrite lookup_insert in D. inv D. inv H7.
-      * put (lookup ι : ProcessPool -> _) on H3 as D.
-        setoid_rewrite lookup_insert in D. inv D. inv H8.
-        - do 2 eexists. split. apply n_refl.
-          admit.
-        - admit.
-        - admit.
-        - admit.
-        - admit.
-        - admit.
-      * admit.
-      * put (lookup ι : ProcessPool -> _) on H3 as D.
-        setoid_rewrite lookup_insert in D. inv D. inv H12.
+      subst. destruct A as [Aeth AΠ]. destruct B' as [Beth BΠ]. inv H.
+      * put (lookup ι : ProcessPool -> _) on H2 as D.
+        setoid_rewrite lookup_insert in D. inv D. inv H4.
+      * put (lookup ι : ProcessPool -> _) on H1 as D.
+        setoid_rewrite lookup_insert in D.
+        unfold etherPop in H5. repeat case_match; try congruence. inv D.
+        inv H5.
+        simpl in Heth. destruct Heth as [? _].
+        exfalso. apply H0. exists ι1. eexists. eassumption.
+      * put (lookup ι : ProcessPool -> _) on H1 as D.
+        setoid_rewrite lookup_insert in D. inv D.
+        destruct_or! H7; subst; inv H5. inv H7.
+        rewrite gset_to_gmap_empty. do 2 eexists. split. apply n_refl.
+        replace (ι ↦ inr ∅ ∥ Π) with (ι ↦ inr ∅ ∥ AΠ). 2: {
+          apply map_eq. intros.
+          put (lookup i : ProcessPool -> _) on H1 as D.
+          destruct (decide (ι = i)).
+          subst. by setoid_rewrite lookup_insert.
+          setoid_rewrite lookup_insert_ne in D; auto.
+          by setoid_rewrite lookup_insert_ne.
+        }
+        apply dead_process_bisim. assumption.
+        intro.
+        apply HΠ. left. intro. by apply not_elem_of_dom in H0.
+      * put (lookup ι : ProcessPool -> _) on H1 as D.
+        setoid_rewrite lookup_insert in D. inv D. inv H11.
     }
     {
       destruct A. simpl in *. destruct B'.
-      inv H1.
+      inv H.
       - assert (p = ι0 ↦ p1 ∥ p) as Eq1. {
           apply map_eq.
-          intro. put (lookup i : ProcessPool -> _) on H4 as HD.
+          intro. put (lookup i : ProcessPool -> _) on H2 as HD.
           destruct (decide (i = ι0)).
           * subst. setoid_rewrite lookup_insert.
             setoid_rewrite lookup_insert in HD.
@@ -243,7 +464,7 @@ Proof with left; by setoid_rewrite lookup_insert.
         + replace (ι0 ↦ p' ∥ prs) with
             (ι ↦ inl ([], RValSeq vs, mb, ∅, flag) ∥ ι0 ↦ p' ∥ p). 2: {
             apply map_eq. intros.
-            put (lookup i : ProcessPool -> _) on H4 as HD.
+            put (lookup i : ProcessPool -> _) on H2 as HD.
             destruct (decide (i = ι)).
             * subst. setoid_rewrite lookup_insert.
               setoid_rewrite lookup_insert_ne; auto.
@@ -256,10 +477,56 @@ Proof with left; by setoid_rewrite lookup_insert.
               - setoid_rewrite lookup_insert_ne in HD; auto.
                 repeat setoid_rewrite lookup_insert_ne; auto.
           }
-          apply IH; try assumption. set_solver.
+          apply IH; try assumption. simpl.
+          ** destruct Heth, H0.
+             assert (ι <> ι'). {
+               intro. apply HΠ. rewrite Eq1.
+               right. do 2 eexists. split. by setoid_rewrite lookup_insert.
+               inv H4; simpl. 1-4: set_solver.
+               apply elem_of_union_list. exists ({[ι']} ∪ usedPIDsVal reason).
+               split. 2: set_solver.
+               apply elem_of_elements, elem_of_map_to_set.
+               do 2 eexists. split. eassumption. reflexivity.
+             }
+             assert (ι ∉ usedPIDsSignal t). {
+               intro. apply HΠ. rewrite Eq1.
+               right. do 2 eexists. split. by setoid_rewrite lookup_insert.
+               inv H4; simpl. 1-4: set_solver.
+               apply elem_of_union_list. exists ({[ι']} ∪ usedPIDsVal reason).
+               split. 2: set_solver.
+               apply elem_of_elements, elem_of_map_to_set.
+               do 2 eexists. split. eassumption. reflexivity.
+             }
+             split. 2: split.
+             -- intro. apply isTargetedEther_etherAdd_rev in H6. congruence.
+                by auto.
+             -- intros. destruct (decide ((ι0, ι') = (ιs, ιd))).
+                ++ inv e0. unfold etherAdd in H6.
+                   case_match; setoid_rewrite lookup_insert in H6; inv H6.
+                   2: set_solver.
+                   rewrite flat_union_app. apply H0 in H7. set_solver.
+                ++ unfold etherAdd in H6.
+                   case_match; setoid_rewrite lookup_insert_ne in H6; auto; inv H6.
+                   all: by apply H0 in H9.
+             -- intros. unfold etherAdd in H6.
+                case_match; setoid_rewrite lookup_insert_ne in H6.
+                2,4: intro X; inv X; lia.
+                all: by apply H1 in H6.
+          ** simpl.
+             rewrite Eq1 in HΠ.
+             eapply not_isUsedPool_step. exact HΠ.
+             2: apply n_send; eassumption. simpl. intro.
+             apply HΠ. right. do 2 eexists. split. by setoid_rewrite lookup_insert.
+             inv H4; simpl in H. 1-4: set_solver. simpl.
+             apply elem_of_union_list. exists ({[ι']} ∪ usedPIDsVal reason). split.
+             2: set_solver.
+             apply elem_of_elements, elem_of_map_to_set. do 2 eexists; split.
+             eassumption. reflexivity.
+         Unshelve.
+          all: exact ∅.
       - assert (p = ι0 ↦ p1 ∥ p) as Eq1. {
           apply map_eq.
-          intro. put (lookup i : ProcessPool -> _) on H3 as HD.
+          intro. put (lookup i : ProcessPool -> _) on H1 as HD.
           destruct (decide (i = ι0)).
           * subst. setoid_rewrite lookup_insert.
             setoid_rewrite lookup_insert in HD.
@@ -272,7 +539,7 @@ Proof with left; by setoid_rewrite lookup_insert.
         + replace (ι0 ↦ p' ∥ prs) with
             (ι ↦ inl ([], RValSeq vs, mb, ∅, flag) ∥ ι0 ↦ p' ∥ p). 2: {
             apply map_eq. intros.
-            put (lookup i : ProcessPool -> _) on H3 as HD.
+            put (lookup i : ProcessPool -> _) on H1 as HD.
             destruct (decide (i = ι)).
             * subst. setoid_rewrite lookup_insert.
               setoid_rewrite lookup_insert_ne; auto.
@@ -285,10 +552,77 @@ Proof with left; by setoid_rewrite lookup_insert.
               - setoid_rewrite lookup_insert_ne in HD; auto.
                 repeat setoid_rewrite lookup_insert_ne; auto.
           }
-          apply IH; try assumption. set_solver.
+          apply IH; try assumption.
+          ** simpl. destruct Heth, H0.
+             split. 2: split.
+             -- intro. eapply isTargetedEther_etherPop_rev in H3. 2: eassumption.
+                congruence.
+             -- intros. unfold etherPop in H5; repeat case_match; try congruence.
+                inv H5. destruct (decide ((ι2, ι0) = (ιs, ιd))).
+                ++ inv e0. setoid_rewrite lookup_insert in H3. inv H3.
+                   apply H0 in H4. set_solver.
+                ++ setoid_rewrite lookup_insert_ne in H3; auto.
+                   by apply H0 in H3.
+             -- intros. unfold etherPop in H5; repeat case_match; try congruence.
+                inv H5. destruct (decide ((ι2, ι0) = (ι, ιd))).
+                ++ inv e0. setoid_rewrite lookup_insert in H3. inv H3.
+                   apply H2 in H4. set_solver.
+                ++ setoid_rewrite lookup_insert_ne in H3; auto.
+                   by apply H2 in H3.
+          ** simpl.
+             intro. rewrite Eq1 in HΠ.
+             unfold etherPop in H5. repeat case_match; try congruence. inv H5.
+             destruct Heth, H3.
+             assert (ι0 <> ι). {
+               intro. subst. apply HΠ...
+             }
+             assert (ι ∉ usedPIDsSignal t). {
+               intro. apply H3 in H0. set_solver.
+             }
+             apply H3 in H0 as P.
+             inv H7.
+             -- apply HΠ.
+                clear -H6 H H5. unfold mailboxPush in H. destruct mb0 ; simpl in *.
+                apply isUsedPool_insert_1 in H as [|[|]]. 2: congruence.
+                all: apply isUsedPool_insert_2.
+                1: by left.
+                do 2 right. simpl in H. rewrite flat_union_app in H. set_solver.
+             -- congruence.
+             -- apply HΠ.
+                clear -H6 H H5 H13.
+                apply isUsedPool_insert_1 in H as [|[|]]. 2: congruence.
+                all: apply isUsedPool_insert_2.
+                1: by left.
+                do 2 right. simpl in H.
+                apply elem_of_union_list in H. destruct_hyps.
+                apply elem_of_elements, elem_of_map_to_set in H. destruct_hyps.
+                subst. apply lookup_gset_to_gmap_Some in H as [? ?]. subst.
+                destruct_or!; destruct_and!; subst; simpl in *; set_solver.
+             -- apply HΠ. assert (ι <> ι2) as X. {
+                  intro. subst. apply H4 in H0 as [_ ?]. clear -H0. set_solver.
+                }
+                clear -H6 H H5 X.
+                apply isUsedPool_insert_1 in H as [|[|]]. 2: congruence.
+                all: apply isUsedPool_insert_2.
+                1: by left.
+                do 2 right. simpl in H. rewrite flat_union_app in H.
+                simpl in H. set_solver.
+             -- apply HΠ. assert (ι <> ι2) as X. {
+                  intro. subst. apply H4 in H0 as [? _]. clear -H0. set_solver.
+                }
+                clear -H6 H H5 X.
+                apply isUsedPool_insert_1 in H as [|[|]]. 2: congruence.
+                all: apply isUsedPool_insert_2.
+                1: by left.
+                do 2 right. simpl in H. set_solver.
+             -- apply HΠ.
+                apply isUsedPool_insert_1 in H as [|[|]]. 2: congruence.
+                all: apply isUsedPool_insert_2.
+                1: by left.
+                do 2 right. simpl in H. set_solver.
       - assert (p = ι0 ↦ p1 ∥ p) as Eq1. {
           apply map_eq.
-          intro. put (lookup i : ProcessPool -> _) on H3 as HD.
+          intro. put (lookup i : ProcessPool -> _) on H1 as HD.
           destruct (decide (i = ι0)).
           * subst. setoid_rewrite lookup_insert.
             setoid_rewrite lookup_insert in HD.
@@ -301,7 +635,7 @@ Proof with left; by setoid_rewrite lookup_insert.
         + replace (ι0 ↦ p' ∥ Π) with
             (ι ↦ inl ([], RValSeq vs, mb, ∅, flag) ∥ ι0 ↦ p' ∥ p). 2: {
             apply map_eq. intros.
-            put (lookup i : ProcessPool -> _) on H3 as HD.
+            put (lookup i : ProcessPool -> _) on H1 as HD.
             destruct (decide (i = ι)).
             * subst. setoid_rewrite lookup_insert.
               setoid_rewrite lookup_insert_ne; auto.
@@ -314,10 +648,17 @@ Proof with left; by setoid_rewrite lookup_insert.
               - setoid_rewrite lookup_insert_ne in HD; auto.
                 repeat setoid_rewrite lookup_insert_ne; auto.
           }
-          apply IH; try assumption. set_solver.
+          apply IH; try assumption.
+          ** simpl.
+             rewrite Eq1 in HΠ.
+             eapply not_isUsedPool_step. exact HΠ.
+             2: apply n_other; eassumption.
+             destruct_or! H7; subst; set_solver.
+         Unshelve.
+          all: exact ∅.
       - assert (p = ι0 ↦ p1 ∥ p) as Eq1. {
           apply map_eq.
-          intro. put (lookup i : ProcessPool -> _) on H3 as HD.
+          intro. put (lookup i : ProcessPool -> _) on H1 as HD.
           destruct (decide (i = ι0)).
           * subst. setoid_rewrite lookup_insert.
             setoid_rewrite lookup_insert in HD.
@@ -326,29 +667,26 @@ Proof with left; by setoid_rewrite lookup_insert.
         }
         rewrite Eq1.
         assert (ι' <> ι0) as Hneq1. {
-          intro. subst. apply H8...
+          intro. subst. apply H6...
         }
         assert (ι' <> ι) as Hneq2. {
-          intro. subst. rewrite H3 in H8. apply H8...
+          intro. subst. rewrite H1 in H6. apply H6...
         }
         do 2 eexists. split.
         + eapply n_trans. 2: apply n_refl. eapply n_spawn; try eassumption.
-          rewrite H3, Eq1 in H8.
-          intro. apply H8.
-          destruct H1.
-          ** left. setoid_rewrite lookup_insert_ne; auto.
-          ** destruct_hyps. right.
-             exists x, x0. split. 2: assumption.
-             destruct (decide (x = ι0)).
-             ++ subst. setoid_rewrite lookup_insert_ne; auto.
-             ++ setoid_rewrite lookup_insert_ne. assumption.
-                intro. subst.
-                apply elem_of_dom_2 in H1.
-                apply H. set_solver.
+          rewrite H1, Eq1 in H6.
+          intro. apply H6.
+          apply isUsedPool_insert_2. left.
+          setoid_rewrite delete_notin. assumption.
+          apply not_elem_of_dom. setoid_rewrite dom_insert_L.
+          assert (ι ∉ dom p). {
+            intro. apply HΠ. left. intro. by apply not_elem_of_dom in H2.
+          }
+          set_solver.
         + replace (ι0 ↦ p' ∥ Π) with
             (ι ↦ inl ([], RValSeq vs, mb, ∅, flag) ∥ ι0 ↦ p' ∥ p). 2: {
             apply map_eq. intros.
-            put (lookup i : ProcessPool -> _) on H3 as HD.
+            put (lookup i : ProcessPool -> _) on H1 as HD.
             destruct (decide (i = ι)).
             * subst. setoid_rewrite lookup_insert.
               setoid_rewrite lookup_insert_ne; auto.
@@ -362,10 +700,68 @@ Proof with left; by setoid_rewrite lookup_insert.
                 repeat setoid_rewrite lookup_insert_ne; auto.
           }
           setoid_rewrite (insert_commute _ ι' ι); auto.
-          apply IH; try assumption. set_solver.
+          assert (ι0 <> ι) as XX. {
+            intro. subst. apply HΠ. rewrite Eq1...
+          }
+          apply IH; try assumption.
+          ** simpl in *.
+             intro. apply HΠ.
+             rewrite H1 in *.
+             apply isUsedPool_insert_1 in H as [|[|]].
+             2: congruence.
+             setoid_rewrite delete_insert_ne in H; auto.
+             apply isUsedPool_insert_1 in H as [|[|]].
+             2: congruence.
+             -- apply not_isUsedPool_insert_1 in H6 as DOM.
+                destruct DOM.
+                setoid_rewrite (delete_notin _ ι') in H. 2: by apply not_elem_of_dom.
+                rewrite Eq1. apply isUsedPool_insert_2. by left.
+             -- rewrite Eq1. right. exists ι0, p1. split. by setoid_rewrite lookup_insert.
+                inv H11; simpl in *; set_solver.
+             -- rewrite Eq1. right. exists ι0, p1. split. by setoid_rewrite lookup_insert.
+                inv H11; simpl in *; case_match; inv H10.
+                2,4: set_solver.
+                ++ repeat rewrite union_empty_r_L in H.
+                   rewrite union_empty_l_L in H.
+                   simpl in H. apply subst_usedPIDs in H; simpl in *.
+                   destruct H; destruct_hyps. clear-H; set_solver.
+                   apply list_subst_idsubst_inl in H.
+                   apply elem_of_app in H as [|].
+                   *** apply elem_of_map_iff in H; destruct_hyps. destruct x1, p0. subst.
+                       simpl in H2. apply elem_of_union in H2 as [|]. 2: clear-H; set_solver.
+                       assert (ι ∈ flat_union (λ x : nat * nat * Exp, usedPIDsExp x.2) ext). {
+                         apply elem_of_flat_union. eexists; split; try eassumption.
+                       }
+                       clear -H2. set_solver.
+                   *** eapply mk_list_usedPIDs in H4.
+                       assert (ι ∈ flat_union usedPIDsVal l). {
+                         apply elem_of_flat_union. eexists; split; eassumption.
+                       }
+                       clear -H3 H4. set_solver.
+                ++ repeat rewrite union_empty_r_L in H.
+                   rewrite union_empty_l_L in H.
+                   simpl in H. apply elem_of_union in H as [H | H].
+                   2: {
+                     clear -H XX. set_solver.
+                   }
+                   apply subst_usedPIDs in H; simpl in *.
+                   destruct H; destruct_hyps. clear-H; set_solver.
+                   apply list_subst_idsubst_inl in H.
+                   apply elem_of_app in H as [|].
+                   *** apply elem_of_map_iff in H; destruct_hyps. destruct x1, p0. subst.
+                       simpl in H2. apply elem_of_union in H2 as [|]. 2: clear-H; set_solver.
+                       assert (ι ∈ flat_union (λ x : nat * nat * Exp, usedPIDsExp x.2) ext). {
+                         apply elem_of_flat_union. eexists; split; try eassumption.
+                       }
+                       clear -H2. set_solver.
+                   *** eapply mk_list_usedPIDs in H4.
+                       assert (ι ∈ flat_union usedPIDsVal l). {
+                         apply elem_of_flat_union. eexists; split; eassumption.
+                       }
+                       clear -H4 H3. set_solver.
     }
-Admitted.
-Set Guard Checking. *)
+Qed.
+Set Guard Checking.
 
 Theorem sequential_to_node :
   forall k fs e fs' e', ⟨fs, e⟩ -[k]-> ⟨fs', e'⟩ ->
@@ -633,6 +1029,9 @@ Hypothesis l_is_proper : mk_list l = Some l'.
 Hypothesis f_closed : forall v, VALCLOSED v -> VALCLOSED (f v).
 Hypothesis l_closed : VALCLOSED l.
 Hypothesis (l_is_free_of_PIDs : usedPIDsVal (meta_to_cons l') = ∅).
+(* These should be rephrased as properties of `f` + l_is_free_of_PIDs *)
+Hypothesis (Hfmeta1 : forall idx, usedPIDsVal (meta_to_cons (map f (take idx l'))) = ∅).
+Hypothesis (Hfmeta2 : forall idx, usedPIDsVal (meta_to_cons (map f (drop idx l'))) = ∅).
 
 Open Scope string_scope.
 
@@ -1886,7 +2285,6 @@ Opaque map_clos.
         eexists. exists []. split. apply n_refl.
         apply barbedBisim_sym.
         
-        (* child terminates - TODO - this is wrong - create a helper to it  *)
         eapply barbedBisim_trans.
         {
           (* eapply normalisation_τ_many_bisim.
@@ -2118,8 +2516,32 @@ Opaque map_clos.
                                  [])]))])], RBox, emptyBox, ∅, false) ∥ ∅)) as HH.
           apply HH; clear HH.                    (* TODO: bug? Direct 
                                                    apply does not work here*)
-          - simpl; setoid_rewrite dom_insert_L. set_solver.
-          - simpl. set_solver.
+          
+          (* Restiction is used here: PIDs cannot appear in the mapped
+             list, because otherwise the helper lemma could not be used *)
+          - simpl in *. split. 2: split.
+            + intro Y. destruct Y as [ιs [l'' Y]].
+              unfold etherAdd in Y. setoid_rewrite lookup_empty in Y.
+              setoid_rewrite lookup_insert_ne in Y. 2: intro YY; inv YY; lia.
+              by setoid_rewrite lookup_empty in Y.
+            + intros * Y. unfold etherAdd in Y. setoid_rewrite lookup_empty in Y.
+              apply lookup_insert_Some in Y as [[? ?]|].
+              ** inv H0. simpl. by rewrite Hfmeta1.
+              ** destruct H0. set_solver.
+            + intros * Y. unfold etherAdd in Y. setoid_rewrite lookup_empty in Y.
+              apply lookup_insert_Some in Y as [[? ?]|].
+              ** inv H0. clear. set_solver.
+              ** set_solver.
+          - simpl in *. intro Y.
+            apply isUsedPool_insert_1 in Y as [|[|]].
+            + destruct H0. set_solver. destruct_hyps. set_solver.
+            + congruence.
+            + simpl in *.
+              assert (usedPIDsVal (meta_to_cons (map f (drop idx l'))) = ∅). {
+                apply Hfmeta2.
+              }
+              rewrite H1 in H0. set_solver.
+          - assumption.
         }
       (* parent receives *)
       constructor.
@@ -3293,8 +3715,29 @@ Opaque map_clos.
                                                   EApp (˝ VFunId (3, 0)) [])]))]))) [])])],
         RValSeq [VLit "infinity"], emptyBox, ∅, false) ∥ ∅)) as HH.
             apply HH; clear HH.
-            - setoid_rewrite dom_insert_L. set_solver.
-            - set_solver.
+            - simpl in *. split. 2: split.
+              + intro Y. destruct Y as [ιs [l'' Y]].
+                unfold etherAdd in Y. setoid_rewrite lookup_empty in Y.
+                setoid_rewrite lookup_insert_ne in Y. 2: intro YY; inv YY; lia.
+                by setoid_rewrite lookup_empty in Y.
+              + intros * Y. unfold etherAdd in Y. setoid_rewrite lookup_empty in Y.
+                apply lookup_insert_Some in Y as [[? ?]|].
+                ** inv H0. simpl. by rewrite Hfmeta1.
+                ** destruct H0. set_solver.
+              + intros * Y. unfold etherAdd in Y. setoid_rewrite lookup_empty in Y.
+                apply lookup_insert_Some in Y as [[? ?]|].
+                ** inv H0. clear. set_solver.
+                ** set_solver.
+            - simpl in *. intro Y.
+              apply isUsedPool_insert_1 in Y as [|[|]].
+              + destruct H0. set_solver. destruct_hyps. set_solver.
+              + congruence.
+              + simpl in *.
+                assert (usedPIDsVal (meta_to_cons (map f (drop idx l'))) = ∅). {
+                  apply Hfmeta2.
+                }
+                rewrite H1 in H0. set_solver.
+            - assumption.
           }
           (* parent receives *)
           constructor.
